ECCA/continuations_lemmas.v
@@ -5,11 +5,32 @@ Require Import String.
 
 Open Scope ECCA_scope.
 
+Lemma het_compose_val (K: cont) (M: exp): isVal M -> het_compose K M = fill_hole M K.
+Proof.
+intros. inversion H; rewrite het_compose_equation; auto.
+Qed.
+
+Hint Resolve het_compose_val. 
+
+Lemma het_compose_comp (K: cont) (M: exp): isComp M -> het_compose K M = fill_hole M K.
+Proof.
+intros. inversion H; auto; rewrite het_compose_equation; auto.
+Qed.
+Hint Rewrite het_compose_comp.
+
+Lemma het_compose_hole (M: exp): het_compose Hole M = M.
+Proof. induction M using term_ind; try (rewrite het_compose_equation; auto; fail).
++ rewrite het_compose_equation. rewrite H. names. tauto.
++ rewrite het_compose_equation. rewrite IHM2. rewrite IHM3. tauto.
+Qed.
+Hint Rewrite het_compose_hole.
+
 Lemma fill_hole_comp_preserves_conf (e: exp) (K: cont) : cont_is_ANF K -> isComp e -> 
 isConf (fill_hole e K).
 Proof.
 intros. destruct K; cbn; auto.
 Qed.
+Hint Resolve fill_hole_comp_preserves_conf.
 
 
 
@@ -33,46 +54,51 @@ induction ANF_val_conf_comp_comb with (P:=P) (P0:=P0) (P1:=P1); auto.
   - apply H0; try apply open_ANF_iff; auto. apply wk_ANF_iff. apply H1.
 + unfold P, P0. intros. rewrite het_compose_equation. apply If; auto. 
 Qed.
+Hint Resolve het_compose_preserves_ANF.
 
-
-Lemma cont_compose_fill_het_compose (x: name) (K K' : cont) (N : exp) (PN: isComp N) (PK: cont_is_ANF K) (PK': cont_is_ANF K'):
-  (het_compose K (fill_hole N K') (fill_hole_preserves_ANF _ _ PK' PN)) = (fill_hole N (cont_compose K K' PK')).
+Lemma het_compose_preserves_conf (e: @exp 0) (i: isConf e): 
+forall K, (cont_is_ANF K -> isConf (het_compose K e)).
 Proof.
-  intros. destruct K'.
-+  cbn. destruct PK'.
-+  cbn. auto..
-+  cbn. rewrite het_compose_r_equation. reflexivity.
-Qed. 
+intros. pose het_compose_preserves_ANF. destruct a. destruct H1. apply H1; auto. 
+Qed.
+Hint Resolve het_compose_preserves_conf.
 
-Require Import Coq.Program.Equality.
-
-
-
-Corollary close_open_id_conf {V x} (M: @conf (S V)): (@close_conf V x (@open_conf V x M)) = M.
-Admitted.
-
-Lemma het_compose_empty_hole (x: name) (M: conf) :
-  (het_compose_r rHole M x) = M.
-Proof.
-  induction M using conf_open_ind.
-  + rewrite het_compose_r_equation. cbn. reflexivity.
-  + rewrite het_compose_r_equation. cbn. rewrite H. cbn. rewrite close_open_id_conf. reflexivity.
-  + rewrite het_compose_r_equation. cbn. rewrite IHM1. rewrite IHM2. reflexivity.
+Lemma cont_compose_preserves_ANF (K K': cont):
+cont_is_ANF K -> cont_is_ANF K' -> cont_is_ANF (cont_compose K K').
+Proof. intros. unfold cont_is_ANF in *. destruct K; destruct K'.
++ auto.
++ cbn. apply close_ANF_iff. rewrite het_compose_hole. apply open_ANF_iff. auto.
++ auto.
++ cbn. apply close_ANF_iff. apply het_compose_preserves_conf. apply open_ANF_iff. auto.
+  cbn. apply open_ANF_iff. apply wk_ANF_iff. auto.
 Qed.
 
+Lemma cont_compose_fill_het_compose (x: name) (K K' : cont) (N : exp) (PN: isComp N) (PK: cont_is_ANF K) (PK': cont_is_ANF K'):
+  (het_compose K (fill_hole N K')) = (fill_hole N (cont_compose K K')).
+Proof.
+  intros. destruct K'.
++  cbn. rewrite het_compose_comp; auto.
++  cbn. rewrite het_compose_equation. auto.
+Qed. 
+Hint Resolve cont_compose_preserves_ANF.
+Require Import Coq.Program.Equality.
+
 Open Scope string.
-Lemma K_compat (g: env) (K : cont_r) (e1 e2 : exp) :
+Lemma K_compat (g: env) (K : cont) (e1 e2 : exp) :
   (RedClos g e1 e2) ->
-  (Equiv g (fill_hole e1 (unrestrict_cont K))) (fill_hole e2 (unrestrict_cont K)).
+  (Equiv g (fill_hole e1 K)) (fill_hole e2 K).
 Proof.
   intros. destruct K.
   + simpl. eapply aE_Step. apply H. apply R_Refl.
-  + simpl. eapply aE_Step.  apply R_CongLet with (x:="x") (A:=Bool).
-    apply H. apply R_Refl. apply R_Refl.
+  + simpl. eapply aE_Step.
+     - eapply R_CongLet with (x:="x") (A:=eUni uProp). (*TODO: This A is arbitrary...*)
+       * apply H.
+       * apply R_Refl.
+     - apply R_Refl.
 Qed.
 
-Lemma bind_commutes_over_fill_hole (g: env) (K : cont_r) (n m : exp) :
-  (Equiv g (bind n (fill_hole m unrestrict_cont (wk_cont K)))) (fill_hole (bind n m) (unrestrict_cont K))).
+(*Lemma bind_commutes_over_fill_hole (g: env) (K : cont) (n m : exp):
+  (Equiv g (bind n (fill_hole m wk_cont K))) (fill_hole (bind n m) K).
 Proof.
   destruct K.
   + simpl. eapply aE_Step; apply R_Refl.
@@ -81,10 +107,10 @@ Proof.
     * eapply aE_Step. apply R_RedR. apply R_Let. apply R_Refl.
     * apply equiv_sym. eapply equiv_trans. apply H. apply equiv_sym.
       (*don't think bind (bind n m) B = (bind n (bind m B)) *)
-Admitted.
+Admitted.*)
 
-Lemma fill_hole_over_branches (g: env) (K : cont_r) (v: val) (m1 m2 : conf) :
-  (Equiv g (eIf v (fill_hole m1 (unrestrict_cont K)) (fill_hole m2 (unrestrict_cont K))) (fill_hole (If v m1 m2) (unrestrict_cont K))).
+Lemma fill_hole_over_branches (g: env) (K : cont) (v m1 m2: exp) (i: isConf (eIf v m1 m2)) :
+  (Equiv g (eIf v (fill_hole m1 K) (fill_hole m2 K)) (fill_hole (eIf v m1 m2) K)).
 Proof.
   destruct K.
   + unfold unrestrict_cont. simpl. eapply aE_Step; apply R_Refl.
